imp/IMem0.v
@@ -1,0 +1,129 @@
+Require Import Coqlib.
+Require Import ITreelib.
+Require Import Universe.
+Require Import STS.
+Require Import Behavior.
+Require Import ModSem.
+Require Import Skeleton.
+Require Import PCM.
+
+Generalizable Variables E R A B C X Y Σ.
+
+Set Implicit Arguments.
+Set Typeclasses Depth 5.
+
+
+
+
+
+
+
+
+Section PROOF.
+  Let memRA: URA.t := (RA.excl Mem.t).
+  Context `{@GRA.inG memRA Σ}.
+  Let GURA: URA.t := GRA.to_URA Σ.
+  Local Existing Instance GURA.
+
+  Compute (URA.car (t:=memRA)).
+
+  Definition allocF_parg (args: list val): option Z :=
+    match args with
+    | [Vint sz] => Some sz
+    | _ => None
+    end
+  .
+
+  Definition allocF: list val -> itree Es val :=
+    fun varg =>
+      mp0 <- trigger (PGet);;
+      m0 <- mp0↓?;;
+      `sz: Z <- (allocF_parg varg)?;;
+      let (blk, m1) := Mem.alloc m0 sz in
+      trigger (PPut m1↑);;
+      Ret (Vptr blk 0)
+  .
+
+  Definition freeF_parg (args: list val): option (block * Z) :=
+    match args with
+    | [Vptr b ofs] => Some (b, ofs)
+    | _ => None
+    end
+  .
+
+  Definition freeF: list val -> itree Es val :=
+    fun varg =>
+      mp0 <- trigger (PGet);;
+      m0 <- mp0↓?;;
+      '(b, ofs) <- (freeF_parg varg)?;;
+      m1 <- (Mem.free m0 b ofs)?;;
+      trigger (PPut m1↑);;
+      Ret (Vint 0)
+  .
+
+  Definition loadF_parg (args: list val): option (block * Z) :=
+    match args with
+    | [Vptr b ofs] => Some (b, ofs)
+    | _ => None
+    end
+  .
+
+  Definition loadF: list val -> itree Es val :=
+    fun varg =>
+      mp0 <- trigger (PGet);;
+      m0 <- mp0↓?;;
+      '(b, ofs) <- (loadF_parg varg)?;;
+      v <- (Mem.load m0 b ofs)?;;
+      Ret v
+  .
+
+  Definition storeF_parg (args: list val): option (block * Z * val) :=
+    match args with
+    | [Vptr b ofs; v] => Some (b, ofs, v)
+    | _ => None
+    end
+  .
+
+  Definition storeF: list val -> itree Es val :=
+    fun varg =>
+      mp0 <- trigger (PGet);;
+      m0 <- mp0↓?;;
+      '(b, ofs, v) <- (storeF_parg varg)?;;
+      m1 <- (Mem.store m0 b ofs v)?;;
+      trigger (PPut m1↑);;
+      Ret (Vint 0)
+  .
+
+  Definition cmpF_parg (args: list val): option (val * val) :=
+    match args with
+    | [v0; v1] => Some (v0, v1)
+    | _ => None
+    end
+  .
+
+  Definition cmpF: list val -> itree Es val :=
+    fun varg =>
+      mp0 <- trigger (PGet);;
+      m0 <- mp0↓?;;
+      '(v0, v1) <- (cmpF_parg varg)?;;
+      b <- (vcmp m0 v0 v1)?;;
+      if b: bool
+      then Ret (Vint 1%Z)
+      else Ret (Vint 0%Z)
+  .
+
+  Definition IMemSem (sk: Sk.t): ModSem.t :=
+    {|
+      ModSem.fnsems := [("alloc", cfun allocF) ; ("free", cfun freeF) ; ("load", cfun loadF) ; ("store", cfun storeF) ; ("cmp", cfun cmpF)];
+      ModSem.mn := "Mem";
+      ModSem.initial_mr := ε;
+      ModSem.initial_st := (Sk.load_mem sk)↑;
+    |}
+  .
+
+  Definition IMem: Mod.t := {|
+    Mod.get_modsem := IMemSem;
+    Mod.sk := Sk.unit;
+  |}
+  .
+End PROOF.
