imp/IMem01proof.v
@@ -1,0 +1,471 @@
+Require Import IMem0 IMem1 HoareDef SimModSem.
+Require Import Coqlib.
+Require Import Universe.
+Require Import Skeleton.
+Require Import PCM.
+Require Import ModSem Behavior.
+Require Import Relation_Definitions.
+
+(*** TODO: export these in Coqlib or Universe ***)
+Require Import Relation_Operators.
+Require Import RelationPairs.
+From ITree Require Import
+     Events.MapDefault.
+From ExtLib Require Import
+     Core.RelDec
+     Structures.Maps
+     Data.Map.FMapAList.
+Require Import TODOYJ.
+Require Import HTactics Logic YPM.
+
+Generalizable Variables E R A B C X Y.
+
+Set Implicit Arguments.
+
+Local Open Scope nat_scope.
+
+
+
+(*** black + delta --> new_black ***)
+Definition add_delta_to_black `{M: URA.t} (b: Auth.t M) (w: Auth.t _): Auth.t _ :=
+  match b, w with
+  | Auth.excl e _, Auth.frag f1 => Auth.excl (e ⋅ f1) URA.unit
+  | _, _ => Auth.boom
+  end
+.
+
+
+(* Notation "wf n *)
+(* '------------------------------------------------------------------' *)
+(* src0 tgt0 *)
+(* '------------------------------------------------------------------' *)
+(* src1 tgt1 *)
+(* '------------------------------------------------------------------' *)
+(* src2 tgt2" := *)
+(*   (sim_itree wf n (([(_, src0)], src1), src2) (([(_, tgt0)], tgt1), tgt2)) *)
+(*     (at level 60, *)
+(*      format "wf  n '//' *)
+(* '------------------------------------------------------------------' '//' *)
+(* src0 '//' *)
+(* tgt0 '//' *)
+(* '------------------------------------------------------------------' '//' *)
+(* src1 '//' *)
+(* tgt1 '//' *)
+(* '------------------------------------------------------------------' '//' *)
+(* src2 '//' '//' '//' *)
+(* tgt2 '//' *)
+(* "). *)
+(******** TODO: it works in emacs but fails in coqc -- try coq 8.13 and uncomment it ***********)
+
+Lemma repeat_nth_some
+      X (x: X) sz ofs
+      (IN: ofs < sz)
+  :
+    nth_error (repeat x sz) ofs = Some x
+.
+Proof.
+  ginduction sz; ii; ss.
+  - lia.
+  - destruct ofs; ss. exploit IHsz; et. lia.
+Qed.
+
+Lemma repeat_nth_none
+      X (x: X) sz ofs
+      (IN: ~(ofs < sz))
+  :
+    nth_error (repeat x sz) ofs = None
+.
+Proof.
+  generalize dependent ofs. induction sz; ii; ss.
+  - destruct ofs; ss.
+  - destruct ofs; ss. { lia. } hexploit (IHsz ofs); et. lia.
+Qed.
+
+Lemma repeat_nth
+      X (x: X) sz ofs
+  :
+    nth_error (repeat x sz) ofs = if (ofs <? sz) then Some x else None
+.
+Proof.
+  des_ifs.
+  - eapply repeat_nth_some; et. apply_all_once Nat.ltb_lt. ss.
+  - eapply repeat_nth_none; et. apply_all_once Nat.ltb_ge. lia.
+Qed.
+
+
+
+Section AUX.
+  Context {K: Type} `{M: URA.t}.
+  Let RA := URA.pointwise K M.
+
+  Lemma pw_extends (f0 f1: K -> M) (EXT: @URA.extends RA f0 f1): forall k, <<EXT: URA.extends (f0 k) (f1 k)>>.
+  Proof. ii. r in EXT. des. subst. ur. ss. eexists; et. Qed.
+  (* Lemma pw_unfold_wf (f: K -> M): (forall k, URA.wf (f k)) -> @URA.wf RA f. Proof. i. ss. Qed. *)
+
+  (* Lemma empty_wf: forall k, URA.wf ((@URA.unit RA) k). *)
+  (* Proof. ii; ss. eapply URA.wf_unit. Qed. *)
+
+  (* Lemma update_wf: forall `{Dec K} (f: @URA.car RA) k v (WF: URA.wf f) (WF: URA.wf v), URA.wf (update f k v: (@URA.car RA)). *)
+  (* Proof. ii. unfold update. des_ifs; ss. Qed. *)
+
+  Lemma lookup_wf: forall (f: @URA.car RA) k (WF: URA.wf f), URA.wf (f k).
+  Proof. ii; ss. rewrite URA.unfold_wf in WF. ss. Qed.
+
+End AUX.
+
+Ltac Ztac := all_once_fast ltac:(fun H => first[apply Z.leb_le in H|apply Z.ltb_lt in H|apply Z.leb_gt in H|apply Z.ltb_ge in H|idtac]).
+
+Lemma _points_to_hit: forall b ofs v, (_points_to (b, ofs) [v] b ofs) = (Some v).
+Proof. i. rewrite unfold_points_to. ss. des_ifs; bsimpl; des; des_sumbool; subst; Ztac; try lia. rewrite Z.sub_diag. ss. Qed.
+
+Lemma _points_to_miss: forall b ofs b' ofs' (MISS: b <> b' \/ ofs <> ofs') v, (_points_to (b, ofs) [v] b' ofs') = ε.
+Proof. i. rewrite unfold_points_to. ss. des_ifs; bsimpl; des; des_sumbool; subst; Ztac; try lia. Qed.
+
+Lemma _points_to_disj: forall b0 ofs0 v0 b1 ofs1 v1,
+    URA.wf (_points_to (b0, ofs0) [v0] ⋅ _points_to (b1, ofs1) [v1]) -> b0 <> b1 \/ ofs0 <> ofs1.
+Proof.
+  ii. do 2 ur in H. specialize (H b0 ofs0). rewrite _points_to_hit in H.
+  rewrite unfold_points_to in H. ss. ur in H. des_ifs_safe. des_ifs; bsimpl; des; des_sumbool; subst; Ztac; try lia.
+  assert(ofs0 = ofs1) by lia. subst. rewrite Z.sub_diag in *. ss.
+Qed.
+
+Lemma dec_true: forall X `{Dec X} (x0 x1: X), x0 = x1 -> ((dec x0 x1): bool) = true.
+Proof. ii. subst. unfold dec. destruct H; ss. Qed.
+
+Lemma dec_false: forall X `{Dec X} (x0 x1: X), x0 <> x1 -> ((dec x0 x1): bool) = false.
+Proof. ii. subst. unfold dec. destruct H; ss. Qed.
+(* Lemma local_update_same *)
+(*       `{M: URA.t} *)
+(*       x0 y0 x1 y1 *)
+(*       (SAME: x0 ⋅ y0 = x1 ⋅ y1) *)
+(*   : *)
+(*     URA.local_update x0 y0 x1 y1 *)
+(* . *)
+(* Proof. *)
+(*   r. ii. des. subst. esplits; et. *)
+(*   - *)
+(* Qed. *)
+
+Section SIMMODSEM.
+
+  Context `{Σ: GRA.t}.
+  Context `{@GRA.inG IMem1.memRA Σ}.
+
+  Let W: Type := ((Σ * Any.t)) * ((Σ * Any.t)).
+  (* Eval compute in (@RA.car (RA.excl Mem.t)). *)
+  Eval compute in (@URA.car IMem1._memRA).
+  Inductive sim_loc: option val -> URA.car (t:=(Excl.t _)) -> Prop :=
+  | sim_loc_present v: sim_loc (Some v) (Some v)
+  | sim_loc_absent: sim_loc None ε
+  .
+
+  Let wf: W -> Prop :=
+    fun '(mrps_src0, mrps_tgt0) =>
+      exists mr_src (mem_tgt: Mem.t),
+        (<<SRC: mrps_src0 = (mr_src, tt↑)>>) /\
+        (<<TGT: mrps_tgt0 = (ε, mem_tgt↑)>>) /\
+        (<<SIM: iHyp (Exists mem_src, Own (GRA.embed ((Auth.black mem_src): URA.car (t:=IMem1.memRA))) **
+                                          (* (Forall b ofs, ⌜~(b = 0 /\ ofs = 0%Z)⌝ -* *)
+                                          (*                  match mem_tgt.(Mem.cnts) b ofs with *)
+                                          (*                  | Some v => Own (GRA.embed ((b, ofs) |-> [v])) *)
+                                          (*                  | None => ⌜True⌝ *)
+                                          (*                  end) *)
+                                          (⌜forall b ofs, sim_loc ((mem_tgt.(Mem.cnts)) b ofs) (mem_src b ofs)⌝)
+                     ) mr_src>>) /\
+        (<<WFTGT: forall b ofs v, mem_tgt.(Mem.cnts) b ofs = Some v -> <<NB: b < mem_tgt.(Mem.nb)>> >>)
+  .
+
+  Hint Resolve sim_itree_mon: paco.
+
+  (* Lemma just_wf `{M: RA.t}: forall (x: @RA.car M), RA.wf x -> @URA.wf (of_RA.t M) (URA.of_RA.just x). *)
+  (* Proof. i; ss. Qed. *)
+
+  (* Opaque of_RA.t. *)
+  (* Opaque URA.auth. *)
+  (* Opaque URA.pointwise. *)
+  Opaque URA.unit.
+
+  Theorem correct: ModPair.sim IMem1.Mem IMem0.IMem.
+  Proof.
+    econs; ss; [|admit "modsem wf"].
+    i. eapply adequacy_lift.
+    econstructor 1 with (wf:=wf); et; swap 2 3.
+    { ss. esplits; ss; et. hexploit gwf_dummy; i. iRefresh.
+      eexists; iRefresh. iSplitP; ss.
+      { eexists. rewrite URA.unit_id. refl. }
+      { ii. destruct (nth_error sk b) eqn:FIND.
+        { destruct p. cbn. des_ifs; try econs. }
+        { cbn. econs. }
+      }
+      { i. ss. eapply nth_error_Some.
+        intros EQ. rewrite EQ in *. ss. }
+    }
+
+    econs; ss.
+    { unfold allocF. init.
+      harg_tac. des_ifs_safe. des. repeat rewrite URA.unit_idl in *. repeat rewrite URA.unit_id in *.
+      iRefresh. iPure PRE. des. clarify. apply Any.upcast_inj in PRE. des; clarify.
+      steps. rewrite Any.upcast_downcast in *. steps.
+      do 2 iDestruct SIM. iPure A.
+      set (blk := (Mem.nb mem_tgt)). rename x into sz. rename x0 into mem_src0.
+
+      astart 0. astop.
+
+      eapply own_upd in SIM; cycle 1; [|rewrite intro_iHyp in SIM; iMod SIM].
+      { eapply GRA.embed_updatable.
+        eapply Auth.auth_alloc2.
+        instantiate (1:=(_points_to (blk, 0%Z) (repeat (Vint 0) sz))).
+        (* instantiate (1:=(fun _b _ofs => if (dec _b blk) && ((0 <=? _ofs) && (_ofs <? Z.of_nat sz))%Z then inl (Some (Vint 0)) else inr tt)). *)
+        iOwnWf SIM. iRefresh.
+        clear - WF WFTGT A.
+        ss. do 2 ur. ii. rewrite unfold_points_to. des_ifs.
+         - bsimpl. des. des_sumbool. subst. hexploit (A blk k0); et. intro T. inv T; [|eq_closure_tac].
+           + exploit WFTGT; et. i; des. lia.
+           + rewrite URA.unit_idl. Ztac. rewrite repeat_length in *. rewrite Z.sub_0_r. rewrite repeat_nth_some; [|lia]. ur. ss.
+         - rewrite URA.unit_id. do 2 eapply lookup_wf. eapply GRA.embed_wf in WF. des. eapply Auth.black_wf; et.
+      }
+      rewrite <- GRA.embed_add in SIM. rewrite own_sep in SIM. iDestruct SIM.
+
+      force_l. eexists. hret_tac SIM A0.
+      - split; [|refl]; iRefresh. eexists; iRefresh. iSplitP; ss.
+      - cbn. esplits; et.
+        + eexists; iRefresh. iSplitL SIM; et. ii.
+          destruct (mem_tgt.(Mem.cnts) blk ofs) eqn:T.
+          { exfalso. exploit WFTGT; et. i; des. lia. }
+          ss. do 2 ur.
+          exploit A; et. rewrite T. intro U. inv U. rewrite unfold_points_to. ss. rewrite repeat_length.
+          destruct (dec b blk); subst; ss.
+          * unfold update. des_ifs_safe. rewrite <- H0. rewrite URA.unit_idl. des_ifs.
+            { rewrite Z.sub_0_r. bsimpl. des. Ztac. rewrite repeat_nth_some; try lia. econs. }
+            { econs. }
+          * rewrite URA.unit_id. unfold update. des_ifs.
+        + clear - WFTGT. i. ss. unfold update in *. des_ifs. exploit WFTGT; et.
+    }
+    econs; ss.
+    { unfold freeF. init.
+      harg_tac. des_ifs_safe. des. repeat rewrite URA.unit_idl in *. repeat rewrite URA.unit_id in *. ss.
+      iRefresh. do 3 iDestruct PRE. iPure PRE. iPure A. clarify. apply Any.upcast_inj in PRE. des; clarify.
+      do 2 iDestruct SIM. iPure A.
+      steps. rewrite Any.upcast_downcast in *. steps.
+
+      astart 0. astop.
+
+      rename n into b. rename z into ofs. rename x0 into mem_src0. rename x into v.
+      iMerge SIM A0. rewrite <- own_sep in SIM. rewrite GRA.embed_add in SIM.
+      iOwnWf SIM. eapply GRA.embed_wf in WF; des.
+      assert(HIT: mem_src0 b ofs = (Some v)).
+      { clear - WF.
+        dup WF. eapply Auth.auth_included in WF. des. eapply pw_extends in WF. eapply pw_extends in WF.
+        rewrite _points_to_hit in WF.
+        eapply Excl.extends in WF; ss. do 2 eapply lookup_wf. eapply Auth.black_wf. eapply URA.wf_mon; et.
+      }
+      set (mem_src1 := fun _b _ofs => if dec _b b && dec _ofs ofs then (ε: URA.car (t:=Excl.t _)) else mem_src0 _b _ofs).
+      assert(WF': URA.wf (mem_src1: URA.car (t:=IMem1._memRA))).
+      { clear - WF. unfold mem_src1. do 2 ur. ii. eapply URA.wf_mon in WF. ur in WF. des.
+        des_ifs; et.
+        - rp; [eapply URA.wf_unit|ss].
+        - do 2 eapply lookup_wf; et.
+      }
+      hexploit (A b ofs); et. rewrite HIT. intro B. inv B.
+      force_r.
+      { unfold Mem.free in *. des_ifs. }
+      rename mem_tgt into mem_tgt0. rename t into mem_tgt1.
+
+      eapply own_upd in SIM; cycle 1; [|rewrite intro_iHyp in SIM; iMod SIM].
+      { eapply GRA.embed_updatable.
+        Local Transparent points_to.
+        eapply Auth.auth_dealloc.
+        instantiate (1:=mem_src1).
+        clear - WF'.
+
+        r. i. rewrite URA.unit_idl.
+        Local Opaque IMem1._memRA.
+        ss. destruct H; clear H. (*** coq bug; des infloops ***) des. clarify.
+        esplits; et.
+        Local Transparent IMem1._memRA.
+        unfold mem_src1. ss.
+        apply func_ext. intro _b. apply func_ext. intro _ofs.
+        des_ifs.
+        - bsimpl; des; des_sumbool; subst.
+          subst mem_src1. do 2 ur in WF'. do 2 spc WF'. des_ifs; bsimpl; des; des_sumbool; ss.
+          clear - H0.
+          do 2 ur in H0.
+          specialize (H0 b ofs). rewrite _points_to_hit in H0. eapply Excl.wf in H0. des; ss.
+        - rewrite unfold_points_to in *. do 2 ur. do 2 ur in H0.
+          bsimpl. des_ifs; bsimpl; des; des_sumbool; subst; Ztac; try lia; try rewrite URA.unit_idl; try refl.
+      }
+      steps. iRefresh. force_l. eexists. hret_tac SIM (@URA.unit Σ).
+      { split; [|refl]. ss. }
+      { ss. esplits; ss; et.
+        - eexists mem_src1; iRefresh. iSplitP; ss. ii.
+          { unfold Mem.free in _UNWRAPU. des_ifs. ss.
+            subst mem_src1. ss.
+            destruct (classic (b = b0 /\ ofs = ofs0)); des; clarify.
+            - unfold update. des_ifs. econs.
+            - des_ifs.
+              { Psimpl. bsimpl; des; des_sumbool; ss; clarify. }
+              replace (update (Mem.cnts mem_tgt0) b (update (Mem.cnts mem_tgt0 b) ofs None) b0 ofs0) with
+                  (Mem.cnts mem_tgt0 b0 ofs0); cycle 1.
+              { unfold update. des_ifs. Psimpl. des_ifs; bsimpl; des; des_sumbool; ss; clarify. }
+              et.
+          }
+        - clear - _UNWRAPU WFTGT. ii. unfold Mem.free in *. des_ifs. ss.
+          unfold update in *. des_ifs; eapply WFTGT; et.
+      }
+    }
+    econs; ss.
+    { unfold loadF. init.
+      harg_tac. des_ifs_safe. des. repeat rewrite URA.unit_idl in *. repeat rewrite URA.unit_id in *. ss.
+      iRefresh. do 2 iDestruct PRE. iPure PRE. iPure A. clarify. apply Any.upcast_inj in PRE. des; clarify.
+      do 2 iDestruct SIM. iPure A.
+      steps. rewrite Any.upcast_downcast in *. steps.
+
+      astart 0. astop.
+      rename n into b. rename z into ofs. rename x into mem_src0.
+      iMerge SIM A0. rewrite <- own_sep in SIM. rewrite GRA.embed_add in SIM. iOwnWf SIM.
+      assert(T: mem_src0 b ofs = (Some v)).
+      { clear - WF.
+        apply GRA.embed_wf in WF. des; ss. dup WF.
+        eapply Auth.auth_included in WF. des.
+        eapply pw_extends in WF. eapply pw_extends in WF. rewrite _points_to_hit in WF.
+        des; ss. eapply Excl.extends in WF; ss. do 2 eapply lookup_wf. eapply Auth.black_wf. eapply URA.wf_mon; et.
+      }
+      exploit A; et. intro U. rewrite T in U. inv U; ss. unfold Mem.load.
+      rewrite <- GRA.embed_add in SIM. rewrite own_sep in SIM. iDestruct SIM.
+      force_r; ss. clarify. steps. force_l. esplits.
+      hret_tac SIM A0.
+      { split; [|refl]; ss; iRefresh. iSplitP; ss. }
+      { ss. esplits; eauto. eexists; iRefresh. iSplitP; ss; et. }
+    }
+    econs; ss.
+    { unfold storeF. init.
+      harg_tac. des_ifs_safe. des. repeat rewrite URA.unit_idl in *. repeat rewrite URA.unit_id in *. ss.
+      iRefresh. do 3 iDestruct PRE. iPure PRE. iPure A. clarify. apply Any.upcast_inj in PRE. des; clarify.
+      do 2 iDestruct SIM. iPure A.
+      steps. rewrite Any.upcast_downcast in *. steps.
+
+      astart 0. astop.
+      rename n into b. rename z into ofs. rename x0 into mem_src0. rename x into v0. rename v into v1.
+      iMerge SIM A0. rewrite <- own_sep in SIM. rewrite GRA.embed_add in SIM. iOwnWf SIM.
+      assert(T: mem_src0 b ofs = (Some v0)).
+      { clear - WF.
+        apply GRA.embed_wf in WF. des; ss. dup WF.
+        eapply Auth.auth_included in WF. des.
+        eapply pw_extends in WF. eapply pw_extends in WF. rewrite _points_to_hit in WF.
+        des; ss.
+        eapply Excl.extends in WF; ss. do 2 eapply lookup_wf. eapply Auth.black_wf. eapply URA.wf_mon; et.
+      }
+      exploit A; et. intro U. rewrite T in U. inv U; ss. unfold Mem.store. des_ifs. steps.
+      set (mem_src1 := fun _b _ofs => if dec _b b && dec _ofs ofs then (Some v1: URA.car (t:=Excl.t _)) else mem_src0 _b _ofs).
+      eapply GRA.embed_wf in WF; des.
+      assert(WF': URA.wf (mem_src1: URA.car (t:=IMem1._memRA))).
+      { clear - WF. unfold mem_src1. do 2 ur. ii. eapply URA.wf_mon in WF. ur in WF. des.
+        des_ifs; et.
+        - bsimpl; des; des_sumbool; subst. ur; ss.
+        - do 2 eapply lookup_wf; et.
+      }
+      eapply own_upd in SIM; cycle 1; [|rewrite intro_iHyp in SIM; iMod SIM].
+      { eapply GRA.embed_updatable. eapply Auth.auth_update with (a':=mem_src1) (b':=_points_to (b, ofs) [v1]); et.
+        clear - wf WF'. ii. des. subst. esplits; et.
+        do 2 ur in WF'. do 2 spc WF'.
+        subst mem_src1. ss. des_ifs; bsimpl; des; des_sumbool; ss.
+        do 2 ur. do 2 (apply func_ext; i). des_ifs.
+        - bsimpl; des; des_sumbool; subst. rewrite _points_to_hit.
+          do 2 ur in WF. do 2 spc WF. rewrite _points_to_hit in WF. eapply Excl.wf in WF. rewrite WF. ur; ss.
+        - bsimpl; des; des_sumbool; rewrite ! _points_to_miss; et.
+      }
+      rewrite <- GRA.embed_add in SIM. rewrite own_sep in SIM. iDestruct SIM. fold (points_to (b,ofs) [v1]) in A0.
+      force_l. eexists.
+      hret_tac SIM A0.
+      { split; [|refl]; iRefresh. ss. }
+      { ss. esplits; eauto.
+        - eexists; iRefresh. iSplitP; ss; et. ii. des_ifs.
+          + bsimpl; des; des_sumbool; subst. do 2 spc A. rewrite Heq in *. rewrite T in *.
+            unfold mem_src1. rewrite ! dec_true; ss. econs.
+          + erewrite f_equal; [apply A|]. unfold mem_src1. des_ifs. bsimpl; des; des_sumbool; subst; ss.
+        - ii. ss. des_ifs.
+          + bsimpl; des; des_sumbool; subst. eapply WFTGT; et.
+          + eapply WFTGT; et.
+      }
+    }
+    econs; ss.
+    { unfold cmpF. init.
+      harg_tac. des_ifs_safe. des. repeat rewrite URA.unit_idl in *. repeat rewrite URA.unit_id in *. ss.
+      iRefresh. do 2 iDestruct SIM. iPure A. do 2 iDestruct PRE. iPure A0. clarify.
+      rename x into mem_src0.
+      assert (VALIDPTR: forall b ofs v (WF: URA.wf ((Auth.black (mem_src0: URA.car (t:=IMem1._memRA))) ⋅ ((b, ofs) |-> [v]))),
+                 Mem.valid_ptr mem_tgt b ofs = true).
+      { clear - A. i. cut (mem_src0 b ofs = Some v).
+        - i. unfold Mem.valid_ptr.
+          specialize (A b ofs). rewrite H in *. inv A. ss.
+        - clear - WF.
+          dup WF.
+          eapply Auth.auth_included in WF. des.
+          eapply pw_extends in WF. eapply pw_extends in WF. rewrite _points_to_hit in WF.
+          des; ss.
+          eapply Excl.extends in WF; ss. do 2 eapply lookup_wf. eapply Auth.black_wf. eapply URA.wf_mon; et.
+      }
+      steps. rewrite Any.upcast_downcast in *. steps.
+      astart 0. astop.
+      Ltac iDestruct H :=
+        match type of H with
+        | iHyp (Exists _, _) _ => destruct H as [? H]; iRefresh
+        | iHyp (_ ** _) _ =>
+          let name0 := fresh "A" in
+          apply sepconj_split in H as [? [? [H [name0 ?]]]]; subst; iRefresh
+        | iHyp (_ ∨ _) _ =>
+          let name0 := fresh "A" in
+          destruct H as [H|name0]; iRefresh
+        end.
+      iMerge SIM A1. rewrite <- own_sep in SIM. iOwnWf SIM. rewrite own_sep in SIM. iDestruct SIM.
+      iDestruct PRE; cycle 1.
+      { iPure A1. des; subst. apply Any.upcast_inj in A1. des; clarify. steps.
+        force_l. eexists. hret_tac SIM A0.
+        { split; [ss; iRefresh|refl]. iSplitP; ss. }
+        { ss. esplits; et. eexists; iRefresh. iSplitP; ss; et. }
+      }
+      iDestruct PRE; cycle 1.
+      { repeat iDestruct A1; subst. iPure A1. iPure A2. iPure A3. subst. apply Any.upcast_inj in A1. des; clarify. steps.
+        rewrite GRA.embed_add in WF. eapply GRA.embed_wf in WF; des.
+        erewrite VALIDPTR; et. ss. rewrite ! dec_true; ss. steps.
+        force_l. eexists. hret_tac SIM A0.
+        { split; [ss; iRefresh|refl]. iSplitP; ss. }
+        { ss. esplits; et. eexists; iRefresh. iSplitP; ss; et. }
+      }
+      iDestruct PRE; cycle 1.
+      { repeat iDestruct A1; subst. iPure A1. iPure A2. iPure A3. subst. apply Any.upcast_inj in A1. des; clarify. steps.
+        rewrite ! GRA.embed_add in WF. eapply GRA.embed_wf in WF; des.
+        erewrite VALIDPTR; et; cycle 1.
+        { rewrite URA.add_assoc in WF. eapply URA.wf_mon in WF; et. }
+        erewrite VALIDPTR; et; cycle 1.
+        { rewrite URA.add_comm with (a:=(x6, x7) |-> [x8]) in WF. rewrite URA.add_assoc in WF. eapply URA.wf_mon in WF; et. }
+        rewrite URA.add_comm in WF. eapply URA.wf_mon in WF. ur in WF; ss.
+        replace (dec x6 x9 && dec x7 x10) with false; cycle 1.
+        { clear - WF.
+          exploit _points_to_disj; et. intro NEQ.
+          des; try (by rewrite dec_false; ss). rewrite dec_false with (x0:=x7); ss. rewrite andb_false_r; ss.
+        }
+        steps. force_l. eexists. hret_tac SIM A0.
+        { split; [ss; iRefresh|refl]. iSplitP; ss. }
+        { ss. esplits; et. eexists; iRefresh. iSplitP; ss; et. }
+      }
+      iDestruct PRE; cycle 1.
+      { repeat iDestruct A1; subst. iPure A1. iPure A2. iPure A3. subst. apply Any.upcast_inj in A1. des; clarify. steps.
+        rewrite GRA.embed_add in WF. eapply GRA.embed_wf in WF; des.
+        erewrite VALIDPTR; et. ss. steps.
+        force_l. eexists. hret_tac SIM A0.
+        { split; [ss; iRefresh|refl]. iSplitP; ss. }
+        { ss. esplits; et. eexists; iRefresh. iSplitP; ss; et. }
+      }
+      iDestruct PRE; cycle 1.
+      { repeat iDestruct PRE; subst. iPure A1. iPure A2. iPure PRE. subst. apply Any.upcast_inj in PRE. des; clarify. steps.
+        rewrite GRA.embed_add in WF. eapply GRA.embed_wf in WF; des.
+        erewrite VALIDPTR; et. ss. steps.
+        force_l. eexists. hret_tac SIM A0.
+        { split; [ss; iRefresh|refl]. iSplitP; ss. }
+        { ss. esplits; et. eexists; iRefresh. iSplitP; ss; et. }
+      }
+    }
+  Qed.
+
+End SIMMODSEM.
